compiler/scheme/scheme_parsingScript.sml
@@ -310,18 +310,11 @@ Termination
   >> gvs[]
 End
 
-Definition static_scope_check_def:
-  static_scope_check p = if static_scope ∅ p
-    then INR p
-    else INL "Not statically scoped or duplicate parameter in lambda or letrec"
-End
-
 Definition parse_to_ast_def:
   parse_to_ast s = do
       lxs <- lexer s;
       e <- parse lxs Nil [];
-      p <- cons_ast (head e);
-      static_scope_check p
+      cons_ast (head e);
     od
 End
 
