compiler/scheme/proofs/scheme_compileCorrectScript.sml
@@ -1,0 +1,85 @@
+open preamble;
+open scheme_astTheory;
+open scheme_semanticsTheory;
+open scheme_to_cakeTheory;
+open scheme_to_cakeProofTheory;
+open primSemEnvTheory;
+open primTypesTheory;
+open ffiTheory;
+open semanticsTheory;
+open evaluateTheory;
+open evaluatePropsTheory;
+open semanticPrimitivesTheory;
+
+val _ = new_theory "scheme_compileCorrect";
+
+Definition v_to_string_def:
+  v_to_string (SBool F) = IO_event (ExtCall "scheme_out") (MAP (n2w o ORD) "#f") [] /\
+  v_to_string (SBool T) = IO_event (ExtCall "scheme_out") (MAP (n2w o ORD) "#t") [] /\
+  v_to_string _ = IO_event (ExtCall "scheme_out") (MAP (n2w o ORD) "other") []
+End
+
+Theorem add_to_sem_env_THE:
+  ! st st' env env' prog .
+    (st', env') = THE (add_to_sem_env (st, env) prog)
+    ==>
+    evaluate_decs st env prog = (st', Rval env')
+Proof
+  rpt strip_tac
+  >> gvs[add_to_sem_env_def]
+  >> Cases_on `evaluate_decs st env prog`
+  >> Cases_on `r`
+  >> gvs[THE_DEF]
+  >> CASE_TAC
+QED
+
+Theorem eval_scheme_env':
+  ! st env .
+    (st, env) = THE (prim_sem_env empty_ffi)
+    ==>
+    evaluate_decs st env (scheme_basis_types ++ scheme_basis ++ [scheme_basis_list; scheme_basis_app]) = (st, Rval scheme_env')
+Proof
+  rpt strip_tac
+  >> EVAL_TAC
+  >> simp[scheme_env'_def]
+  >> simp[add_to_sem_env_def]
+  >> gvs[]
+  >> pop_assum $ simp o single o GSYM
+  >> rpt (pairarg_tac >> gvs[])
+  >> simp[evaluate_decs_append]
+  >> CASE_TAC
+  >> CASE_TAC
+  >> simp[]
+
+  >> CASE_TAC
+  >> CASE_TAC
+  >> simp[Once evaluate_decs_cons]
+
+  >> CASE_TAC
+  >> CASE_TAC
+  >> simp[]
+
+  >> CASE_TAC
+  >> simp[]
+QED
+
+Theorem scheme_semantics_preservation_terminates:
+  ! prog cml_prog v st env ffi .
+    scheme_semantics_prog prog (STerminate v) /\
+    static_scope_check prog = INR prog /\
+    codegen prog = INR cml_prog /\
+    (st, env) = THE (prim_sem_env empty_ffi)
+    ==>
+    semantics_prog st env cml_prog (Terminate Success [v_to_string v])
+Proof
+  (*Somewhere in here, I need a lemma that evaluate st env (...) = (st', Rval scheme_env')*)
+  simp[semantics_prog_def, scheme_semantics_prog_def]
+  >> simp[codegen_def, static_scope_check_def]
+  >> simp[evaluate_prog_with_clock_def]
+  >> rpt strip_tac
+  >> SRULE [] scheme_env'_def
+  >> extend_dec_env_def
+  >> evaluate_decs_append
+QED
+
+val _ = export_theory();
